erasure/theories/EPrimitive.v
@@ -1,0 +1,159 @@
+(* Distributed under the terms of the MIT license. *)
+From MetaCoq.Utils Require Import utils.
+From MetaCoq.Common Require Import Universes Primitive Reflect
+     Environment EnvironmentTyping.
+(* From MetaCoq.Erasure Require Import BasicAst. *)
+From Equations Require Import Equations.
+From Coq Require Import ssreflect.
+From Coq Require Import Uint63 SpecFloat.
+
+Implicit Type term : Set.
+
+Record array_model {term : Set} : Set :=
+  { array_default : term;
+    array_value : list term }.
+Derive NoConfusion for array_model.
+
+Arguments array_model : clear implicits.
+#[global]
+Instance array_model_eqdec {term} (e : EqDec term) : EqDec (array_model term).
+Proof. eqdec_proof. Qed.
+
+(* We use this inductive definition instead of the more direct case analysis
+  [prim_model_of] so that [prim_model] can be used in the inductive definition
+  of terms, otherwise it results in a non-strictly positive definition.
+  *)
+Inductive prim_model (term : Set) : prim_tag -> Set :=
+| primIntModel (i : PrimInt63.int) : prim_model term primInt
+| primFloatModel (f : PrimFloat.float) : prim_model term primFloat
+| primArrayModel (a : array_model term) : prim_model term primArray.
+
+Arguments primIntModel {term}.
+Arguments primFloatModel {term}.
+Arguments primArrayModel {term}.
+
+Derive Signature NoConfusion for prim_model.
+
+Definition prim_model_of (term : Set) (p : prim_tag) : Set :=
+  match p with
+  | primInt => PrimInt63.int
+  | primFloat => PrimFloat.float
+  | primArray => array_model term
+  end.
+
+Definition prim_val term : Set := ∑ t : prim_tag, prim_model term t.
+Definition prim_val_tag {term} (s : prim_val term) := s.π1.
+Definition prim_val_model {term} (s : prim_val term) : prim_model term (prim_val_tag s) := s.π2.
+
+Definition prim_model_val {term} (p : prim_val term) : prim_model_of term (prim_val_tag p) :=
+  match prim_val_model p in prim_model _ t return prim_model_of term t with
+  | primIntModel i => i
+  | primFloatModel f => f
+  | primArrayModel a => a
+  end.
+
+Lemma exist_irrel_eq {A} (P : A -> bool) (x y : sig P) :
+  proj1_sig x = proj1_sig y -> x = y.
+Proof.
+  destruct x as [x p], y as [y q]; simpl; intros ->.
+  now destruct (uip p q).
+Qed.
+
+#[global]
+Instance reflect_eq_Z : ReflectEq Z := EqDec_ReflectEq _.
+
+Import ReflectEq.
+
+Local Obligation Tactic := idtac.
+
+Definition eqb_array {term} {eqt : term -> term -> bool} (x y : array_model term) :=
+   forallb2 eqt x.(array_value) y.(array_value) &&
+   eqt x.(array_default) y.(array_default).
+
+#[program,global]
+Instance reflect_eq_array {term} {req : ReflectEq term}: ReflectEq (array_model term) :=
+  { eqb := eqb_array (eqt := eqb) }.
+Next Obligation.
+  intros term req [] []; cbn. unfold eqb_array. cbn.
+  change (forallb2 eqb) with (eqb (A := list term)).
+  case: eqb_spec => //=. intros ->.
+  case: eqb_spec => //=. intros ->. constructor; auto.
+  all:constructor; congruence.
+Qed.
+
+Equations eqb_prim_model {term} {req : term -> term -> bool} {t : prim_tag} (x y : prim_model term t) : bool :=
+  | primIntModel x, primIntModel y := ReflectEq.eqb x y
+  | primFloatModel x, primFloatModel y := ReflectEq.eqb x y
+  | primArrayModel x, primArrayModel y := eqb_array (eqt:=req) x y.
+
+#[global, program]
+Instance prim_model_reflecteq {term} {req : ReflectEq term} {p : prim_tag} : ReflectEq (prim_model term p) :=
+  {| ReflectEq.eqb := eqb_prim_model (req := eqb) |}.
+Next Obligation.
+  intros. depelim x; depelim y; simp eqb_prim_model.
+  case: ReflectEq.eqb_spec; constructor; subst; auto. congruence.
+  case: ReflectEq.eqb_spec; constructor; subst; auto. congruence.
+  change (eqb_array a a0) with (eqb a a0).
+  case: ReflectEq.eqb_spec; constructor; subst; auto. congruence.
+Qed.
+
+#[global]
+Instance prim_model_eqdec {term} {req : ReflectEq term} : forall p : prim_tag, EqDec (prim_model term p) := _.
+
+Equations eqb_prim_val {term} {req : term -> term -> bool} (x y : prim_val term) : bool :=
+  | (primInt; i), (primInt; i') := eqb_prim_model (req := req) i i'
+  | (primFloat; f), (primFloat; f') := eqb_prim_model (req := req) f f'
+  | (primArray; a), (primArray; a') := eqb_prim_model (req := req) a a'
+  | x, y := false.
+
+#[global, program]
+Instance prim_val_reflect_eq {term} {req : ReflectEq term} : ReflectEq (prim_val term) :=
+  {| ReflectEq.eqb := eqb_prim_val (req := eqb) |}.
+Next Obligation.
+  intros. funelim (eqb_prim_val x y); simp eqb_prim_val.
+  change (eqb_prim_model i i') with (eqb i i').
+  case: ReflectEq.eqb_spec; constructor; subst; auto. intros H; noconf H. cbn in n. auto.
+  constructor. intros H; noconf H; auto.
+  constructor. intros H; noconf H; auto.
+  constructor. intros H; noconf H; auto.
+  change (eqb_prim_model f f') with (eqb f f').
+  case: ReflectEq.eqb_spec; constructor; subst; auto. intros H; noconf H; auto.
+  constructor. intros H; noconf H; auto.
+  constructor. intros H; noconf H; auto.
+  constructor. intros H; noconf H; auto.
+  change (eqb_prim_model a a') with (eqb a a').
+  case: ReflectEq.eqb_spec; constructor; subst; auto. intros H; noconf H; auto.
+Qed.
+
+#[global]
+Instance prim_tag_model_eqdec term {req : ReflectEq term} : EqDec (prim_val term) := _.
+
+(** Printing *)
+
+Definition string_of_prim {term} (soft : term -> string) (p : prim_val term) : string :=
+  match p.π2 return string with
+  | primIntModel f => "(int: " ^ string_of_prim_int f ^ ")"
+  | primFloatModel f => "(float: " ^ string_of_float f ^ ")"
+  | primArrayModel a => "(array:" ^ soft a.(array_default) ^ " , " ^ string_of_list soft a.(array_value) ^ ")"
+  end.
+
+Definition map_array_model {term term'} (f : term -> term') (a : array_model term) : array_model term' :=
+  {| array_default := f a.(array_default);
+     array_value := map f a.(array_value) |}.
+
+Definition map_prim {term term'} (f : term -> term') (p : prim_val term) : prim_val term' :=
+  match p.π2 return prim_val term' with
+  | primIntModel f => (primInt; primIntModel f)
+  | primFloatModel f => (primFloat; primFloatModel f)
+  | primArrayModel a => (primArray; primArrayModel (map_array_model f a))
+  end.
+
+Definition test_array_model {term} (f : term -> bool) (a : array_model term) : bool :=
+  f a.(array_default) && forallb f a.(array_value).
+
+Definition test_prim {term} (f : term -> bool) (p : prim_val term) : bool :=
+  match p.π2 return bool with
+  | primIntModel f => true
+  | primFloatModel f => true
+  | primArrayModel a => test_array_model f a
+  end.
